ber_check_tag fail proof

src/Lib/BCT/Exec.v
@@ -9,20 +9,46 @@ Definition ber_check_tags (td : TYPE_descriptor) (ls : list byte) :
   match decoder_type td with
   | BOOLEAN_t => match ls with
                 | x1::x2::_ => if ((x1 == Byte.one) && (x2 == Byte.one))%byte
-                            then Some (mk_check_tag_rval 2 1 )
+                            then Some (mk_check_tag 2 1 )
                             else None
                 | _ => None
                 end
   | _ => None
   end.
 
-Theorem ber_check_tags_bool_succ : forall td ls,
+Theorem ber_check_tags_bool_res : forall td ls,
     decoder_type td = BOOLEAN_t ->
-    ber_check_tags td ([Byte.one; Byte.one] ++ ls) = 
-    Some (mk_check_tag_rval 2 1).
+    ber_check_tags td ls = Some (mk_check_tag 2 1) 
+    \/ ber_check_tags td ls = None.
+Proof.
+  intros.
+  unfold ber_check_tags; rewrite H.
+  repeat break_match; auto.
+Qed.
+
+Theorem ber_check_tags_bool_Some : forall td ls,
+    decoder_type td = BOOLEAN_t ->
+    ber_check_tags td (Byte.one::Byte.one::ls) = 
+    Some (mk_check_tag 2 1).
 Proof.
   intros.
   unfold ber_check_tags.
   rewrite H.
   reflexivity.
+Qed.
+
+Theorem ber_check_tags_bool_Some_intro : forall td ls,
+    decoder_type td = BOOLEAN_t ->
+    ber_check_tags td ls = Some (mk_check_tag 2 1) ->
+    exists tl, ls = 1%byte::1%byte::tl.
+Proof.
+  intros td ls DT.
+  unfold ber_check_tags.
+  repeat break_match; try discriminate.
+  intros.
+  unfold andb in Heqb; repeat break_match_hyp; try discriminate.
+  pose proof Byte.eq_spec i 1%byte as T; rewrite Heqb0 in T.
+  pose proof Byte.eq_spec i0 1%byte as T1; rewrite Heqb in T1.
+  rewrite T, T1.
+  exists l0; reflexivity.
 Qed.
