src/Primitive/Boolean/Exec.v
@@ -40,8 +40,8 @@ Definition bool_decoder td ls : option (bool * Z) :=
     | [] => None
     | _ => ber_check_tags td ls >>=
                         fun x => let c := tag_consumed x in 
-                              let e := tag_expected x in 
-                              if (Zlength ls - c <? e) || negb (e =? 1) 
+                              let l := tag_length x in 
+                              if (Zlength ls - c <? l) || negb (l =? 1) 
                               then None 
                               else hd_error (skipn (Z.to_nat c) ls) 
                                      >>= fun y => Some (bool_of_byte y, c + 1)
@@ -49,18 +49,16 @@ Definition bool_decoder td ls : option (bool * Z) :=
 
 (* Related lemmas *)
 
-Theorem boolean_dec_res : forall td ls res,
+Theorem boolean_dec_res : forall td ls,
   decoder_type td = BOOLEAN_t ->
-  bool_decoder td [Byte.repr 1; Byte.repr 1; byte_of_bool res] 
-  = Some (res, 3) \/ bool_decoder td ls = None.
+  bool_decoder td ls = None \/ exists res, bool_decoder td ls = Some (res, 3).
 Proof.
   intros.
   unfold bool_decoder, primitive_decoder, ber_check_tags, Byte.one; rewrite H.
-  assert (Byte.repr 1 == Byte.repr 1 = true)%byte as T by reflexivity; 
-    rewrite T; cbn.
-  replace (Pos.to_nat 2) with (2)%nat by reflexivity.
-  do 2 rewrite skipn_cons; rewrite skipn_O; rewrite hd_error_cons.
-  unfold bool_of_byte, byte_of_bool; repeat break_match; try discriminate; auto.
+  repeat break_match; try discriminate; auto.
+  cbn.
+  repeat break_match; try discriminate; auto.
+  right; exists (bool_of_byte i1); reflexivity.
 Qed.
 
 End Decoder.
