src/Correctness/BooleanCorrectness.v
@@ -12,14 +12,13 @@ Theorem der_encoder_correctness : forall td b ls ,
   execErrW (bool_encoder td b) nil = Some ls ->
   DER (BOOLEAN b) ls.
 Proof.
-  intros TD Val Res DT Enc; intros.
-  unfold bool_encoder, primitive_encoder, Exec.der_write_tags
-     in Enc. 
-  rewrite DT in Enc; cbn in Enc.
-  inversion Enc; rename H0 into Res'.
-  replace ([Byte.repr 1; Byte.repr 1; byte_of_bool Val]) with
+  intros TD Val Res DT.
+  rewrite exec_boolean_enc by assumption.
+  intros.
+  inversion H. 
+  replace ([1%byte; 1%byte; byte_of_bool Val]) with
       ([Byte.repr 1] ++ [Byte.repr 1] ++ [byte_of_bool Val]) by reflexivity.
-  destruct Val eqn:V in Enc; subst; repeat econstructor.
+  destruct Val eqn:V; subst; repeat econstructor.
 Qed.
 
 Theorem ber_decoder_correctness : forall td ls b z,
@@ -32,22 +31,24 @@ Proof.
   intros TD ToDec ResB Len DT Dec.
   unfold bool_decoder, Exec.ber_check_tags in Dec; cbn in Dec.
   rewrite DT in Dec; cbn in Dec.
-  destruct ToDec eqn:K1; [congruence|]; 
-    destruct l eqn:K2; [congruence|]; 
-      destruct ((i == 1) && (i0 == 1))%byte; cbn in *; [|congruence]; 
-        destruct (Zlength_aux 2 byte l0 - 2 <? 1); cbn in *; [congruence|].
-  replace (Pos.to_nat 2) with (2)%nat in Dec by reflexivity; 
-    do 2 rewrite skipn_cons in Dec; 
-    rewrite skipn_O in Dec.
-  destruct l0 eqn:K3; cbn in *; [congruence|]; 
-    inversion Dec.
-  replace (Z.to_nat (3 - 1)) with (2)%nat by reflexivity; 
+  repeat break_match_hyp; try discriminate.
+  inversion Heqo.
+  inversion Dec.
+  subst; cbn in *.
+  replace (Pos.to_nat 2) with (2)%nat in Heqo0 by reflexivity; 
+    do 2 rewrite skipn_cons in Heqo0; 
+    rewrite skipn_O in Heqo0.
+  destruct l0 eqn:K3; cbn in *; [congruence|].
+  replace (Pos.to_nat 2) with (2)%nat by reflexivity; 
     do 2 rewrite skipn_cons; rewrite skipn_O; 
       unfold byte_of_bool.
   pose proof Byte.eq_spec i1 (default_byte).
   unfold bool_of_byte.
-  destruct (i1 == default_byte)%byte eqn:K; cbn in *; subst; econstructor.
-  assumption.
+  inversion Heqo0.
+  destruct (i0 == default_byte)%byte eqn:K; cbn in *; subst; 
+    pose proof Byte.eq_spec i0 default_byte; rewrite K in H0.
+  subst; econstructor.
+  econstructor; assumption.
 Qed.
 
 Theorem boolean_roundtrip : forall td ls b z,
@@ -57,8 +58,8 @@ Theorem boolean_roundtrip : forall td ls b z,
     bool_decoder td ls = Some (b, z).
 Proof.
   intros TD ls B z DT Len.
-  unfold execErrW, bool_encoder, primitive_encoder, 
-  Exec.der_write_tags, bool_decoder, 
+  unfold execErrW, bool_encoder, primitive_encoder,
+  Exec.der_write_tags, bool_decoder,
   Exec.ber_check_tags, bool_of_byte; cbn; rewrite DT.
   intros Res; inversion Res as [T]; clear Res; rename T into Res.
   replace (Byte.repr 1 == 1)%byte with true by reflexivity; cbn.
