src/Primitive/Boolean/VstDec.v
@@ -33,19 +33,25 @@ Definition bool_ber_decode_spec : ident * funspec :=
            data_at Tsh (tarray tschar (Zlength buf)) (map Vbyte buf) buf_p;
            data_at Tsh (tptr tvoid) bv_p bv_pp;
            data_at_ Tsh asn_dec_rval_s res_p)
-    POST [tvoid]
+    POST [tvoid] EX p : val * type * list byte,
       PROP ()
       LOCAL ()
       SEP ((* Unchanged by the execution : *)
+           if eq_dec (fst (fst p)) nullval 
+           then emp 
+           else malloc_token Ews (snd (fst p)) (fst (fst p)) * 
+                data_at Ews (tarray tschar 1) (map Vbyte (snd p)) (fst (fst p));
            valid_pointer bv_p;
            data_at Tsh asn_codec_ctx_s ctx ctx_p;
            data_at_ Tsh type_descriptor_s td_p;
            data_at Tsh (tarray tschar (Zlength buf)) (map Vbyte buf) buf_p;
-           data_at Tsh (tptr tvoid) bv_p bv_pp;
+           data_at Tsh (tptr tvoid) (if eq_dec bv_p nullval 
+                                     then fst (fst p) 
+                                     else bv_p) bv_pp;
            (* Changes according to the exec spec *)
            let RC_FAIL := 
                data_at Tsh asn_dec_rval_s (construct_dec_rval 2 0) res_p in
-           if Val.eq bv_p Vnullptr 
+           if eq_dec (fst (fst p)) nullval
            then RC_FAIL 
            else match bool_decoder td buf with
                 | Some (r, c) => 
@@ -56,18 +62,20 @@ Definition bool_ber_decode_spec : ident * funspec :=
 
 Definition if_post1 bv_p v__res__1 v_tmp_error v_length v_rval 
            res_p ctx ctx_p td_p bv_pp buf buf_p size tag_mode := 
-  EX is_inner : bool, EX p : val * type * list byte,
+  EX p : val * type * list byte,
   PROP ()
-  LOCAL (temp _st (if is_inner then fst (fst p) else bv_p); temp _t'11 bv_p;
+  LOCAL (temp _st (if eq_dec bv_p nullval then fst (fst p) else bv_p); 
+         temp _t'11 bv_p;
          lvar __res__1 (Tstruct _asn_dec_rval_s noattr) v__res__1;
          lvar _tmp_error (Tstruct _asn_dec_rval_s noattr) v_tmp_error;
-         lvar _length tint v_length; temp __res res_p; temp _opt_codec_ctx ctx_p;
+         lvar _length tint v_length; temp __res res_p; 
+         temp _opt_codec_ctx ctx_p;
          lvar _rval (Tstruct _asn_dec_rval_s noattr) v_rval;
          temp _td td_p; temp _bool_value bv_pp;
          temp _buf_ptr buf_p; temp _size (Vint (Int.repr size));
          temp _tag_mode (Vint (Int.repr tag_mode)))
   SEP (if eq_dec (fst (fst p)) nullval 
-       then emp 
+       then emp
        else malloc_token Ews (snd (fst p)) (fst (fst p)) * 
             data_at Ews (tarray tschar 1) (map Vbyte (snd p)) (fst (fst p));
        data_at_ Tsh (Tstruct _asn_dec_rval_s noattr) v__res__1;
@@ -77,11 +85,9 @@ Definition if_post1 bv_p v__res__1 v_tmp_error v_length v_rval
        data_at Tsh asn_codec_ctx_s ctx ctx_p;
        data_at_ Tsh type_descriptor_s td_p;
        data_at Tsh (tarray tschar (Zlength buf)) (map Vbyte buf) buf_p;
-       data_at Tsh (tptr tvoid) (if is_inner then fst (fst p) else bv_p) bv_pp;
+       data_at Tsh (tptr tvoid) (if eq_dec bv_p nullval 
+                                 then fst (fst p) else bv_p) bv_pp;
        data_at_ Tsh asn_dec_rval_s res_p).
-
-(*Definition loop_inv1 :=.
-Definition loop_post1 :=.*)
 
 Definition Gprog := ltac:(with_library prog [(_calloc, calloc_spec);
                                               ber_check_tags_spec; 
@@ -92,8 +98,7 @@ Theorem bool_der_encode : semax_body Vprog Gprog
            bool_ber_decode_spec.
 Proof.
   start_function.
-  unfold MORE_COMMANDS.
-  unfold abbreviate.
+  rename H0 into DT.
   repeat forward.
   forward_if (if_post1 bv_p v__res__1 v_tmp_error v_length v_rval res_p ctx 
                        ctx_p td_p bv_pp buf buf_p size tag_mode).
@@ -104,34 +109,43 @@ Proof.
     forward.
     forward.
     forward_if.
-    if_tac; break_let.
-    - cbn in H1; subst.
-      entailer!.
-    - eapply denote_tc_test_eq_split; entailer!.
-    - unfold fst in *; rewrite H4.
+    {
+      if_tac; break_let. 
+      cbn in H0; subst; entailer!.
+      eapply denote_tc_test_eq_split; entailer!.
+    }
+    - (* malloc returned null *)
+      unfold fst in *; rewrite H3.
       rewrite if_true by reflexivity.
       repeat forward.
+      Exists p.
+      rewrite if_true by assumption.
       rewrite if_true by reflexivity.
+      rewrite if_true by assumption.
+      rewrite H3.
       entailer!.
-    - forward.
+    - (* maloc returned non-null value *)
+      forward.
       unfold if_post1.
+      Exists p.
       rewrite if_false by assumption.
-      Exists true p.
-      rewrite if_false by assumption.
+      repeat rewrite if_true by assumption.
       entailer!.
   * (* _st <> NULL *)
     forward.
     unfold if_post1.
-    (* p belongs to inner if, since we didn't reach it, it's uninitialized *)
-    Exists false (nullval, tptr tvoid, buf).
+    Exists (nullval, tptr tvoid, buf).
+    rewrite if_false by assumption.
     rewrite if_true by reflexivity.
+    rewrite if_false by assumption.
     entailer!.
-  * (* after the if *)
+  * (* after the first if *)
     unfold if_post1.
-    Intros is_inner p.
+    Intros p.
     forward_loop 
       (PROP ()
-       LOCAL (temp _st (if is_inner then fst (fst p) else bv_p);
+       LOCAL (temp _st (if eq_dec bv_p nullval 
+                        then fst (fst p) else bv_p);
               lvar __res__1 (Tstruct _asn_dec_rval_s noattr) v__res__1;
               lvar _tmp_error (Tstruct _asn_dec_rval_s noattr)
                 v_tmp_error; lvar _length tint v_length;
@@ -153,12 +167,13 @@ Proof.
             data_at_ Tsh type_descriptor_s td_p;
             data_at Tsh (tarray tschar (Zlength buf)) 
               (map Vbyte buf) buf_p;
-            data_at Tsh (tptr tvoid)
-              (if is_inner then fst (fst p) else bv_p) bv_pp;
+            data_at Tsh (tptr tvoid) (if eq_dec bv_p nullval 
+                                      then fst (fst p) else bv_p) bv_pp;
             data_at_ Tsh asn_dec_rval_s res_p)) 
       break: 
       (PROP ()
-       LOCAL (temp _st (if is_inner then fst (fst p) else bv_p);
+       LOCAL (temp _st (if eq_dec bv_p nullval 
+                        then fst (fst p) else bv_p);
               lvar __res__1 (Tstruct _asn_dec_rval_s noattr) v__res__1;
               lvar _tmp_error (Tstruct _asn_dec_rval_s noattr)
                 v_tmp_error; lvar _length tint v_length;
@@ -180,8 +195,8 @@ Proof.
             data_at_ Tsh type_descriptor_s td_p;
             data_at Tsh (tarray tschar (Zlength buf)) 
               (map Vbyte buf) buf_p;
-            data_at Tsh (tptr tvoid)
-              (if is_inner then fst (fst p) else bv_p) bv_pp;
+            data_at Tsh (tptr tvoid) (if eq_dec bv_p nullval 
+                                      then fst (fst p) else bv_p) bv_pp;
             data_at_ Tsh asn_dec_rval_s res_p)).
     - (* pre-condition = invariant *)
       entailer!.
@@ -189,8 +204,22 @@ Proof.
       forward.
       entailer!.
     - (* after the loop *)
-      forward_call (ctx_p, ctx, td_p, td, nullval, nullval, buf_p, buf, v_rval, 
-                    size, tag_mode, 0, v_length, 0, nullval, 0). 
+      forward_call (ctx_p, ctx, td_p, td, nullval, nullval, buf_p, buf,
+                    v__res__1, size, tag_mode, 0, v_length, 0, nullval, 0). 
+      pose proof Exec.ber_check_tags_bool_res td buf DT as BCT.
+      inversion BCT as [T | T]; rewrite T;
+        unfold construct_dec_rval, tag_length, tag_consumed.
+      2: { (* If ber_check_tags failed *)
+        repeat forward.
+        forward_if; [|discriminate].
+        repeat forward.
+        Exists p.
+        entailer!.
+        break_if. 
+        entailer!.
+        unfold bool_decoder; rewrite T; cbn; destruct buf; entailer!.
+      }
+      (* If ber_check_tags succeded *)
       admit.
 Admitted.
 
